fr.inria.atlanmod.coqtl.coq/core/Metamodel.v
@@ -5,11 +5,12 @@ Require Import core.EqDec.
 Class Metamodel :=
 {
     ModelElement: Type;
+    ModelLink: Type;
     
     elements_eqdec: EqDec ModelElement;
 
     (* Decidable Equality*)
     elements_eqb := eq_b;
 
-    InstanceModel := Model ModelElement;
+    InstanceModel := Model ModelElement ModelLink;
 }.
