fr.inria.atlanmod.coqtl.coq/core/TransformationConfiguration.v
@@ -6,7 +6,10 @@ Class TransformationConfiguration := {
   TargetMetamodel: Metamodel;
 
   SourceModelElement:= @ModelElement SourceMetamodel;
+  SourceModelLink:= @ModelLink SourceMetamodel;
+
   TargetModelElement:= @ModelElement TargetMetamodel;
+  TargetModelLink:= @ModelLink TargetMetamodel;
 
   SourceModel := @InstanceModel SourceMetamodel;
   TargetModel := @InstanceModel TargetMetamodel;
