fr.inria.atlanmod.coqtl.coq/core/modeling/byrule/Certification_ByRuleSemantics.v
@@ -318,7 +318,7 @@ Proof.
 Qed.
 
 Theorem tr_execute_in_links :
-  forall (tr: Transformation) (sm : SourceModel) (tl : TargetModelElement),
+  forall (tr: Transformation) (sm : SourceModel) (tl : TargetModelLink),
     In tl (allModelLinks (execute tr sm)) <->
     (exists (sp : list SourceModelElement),
         In sp (allTuples tr sm) /\
@@ -347,7 +347,7 @@ Proof.
 Qed.
 
 Theorem tr_execute_in :
-  forall (tr: Transformation) (sm : SourceModel) (te : TargetModelElement) (tl : TargetModelElement),
+  forall (tr: Transformation) (sm : SourceModel) (te : TargetModelElement) (tl : TargetModelLink),
     (In te (allModelElements (execute tr sm)) <-> In te (allModelElements (Semantics.execute tr sm)))
     /\ (In tl (allModelLinks (execute tr sm)) <-> In tl (allModelLinks (Semantics.execute tr sm))).
 Proof.
@@ -370,13 +370,13 @@ Instance ByRuleEngine :
   SourceModelReference := SourceModelReference;
   TargetModelElement := TargetModelElement;
   TargetModelClass := TargetModelClass;
-  TargetModelElement := TargetModelElement;
+  TargetModelLink := TargetModelLink;
   TargetModelReference := TargetModelReference;
 
   Transformation := Transformation;
   Rule := Rule;
   OutputPatternElement := OutputPatternElement;
-  OutputPatternNext := OutputPatternNext;
+  OutputPatternLink := OutputPatternLink;
 
   TraceLink := TraceLink;
 
